Finish refactoring substitution lemmas

theories/structural.v
@@ -75,44 +75,44 @@ Qed.
 
 Lemma E_IndCong' Γ P0 P1 (a0 a1 : PTm ) b0 b1 c0 c1 i U :
   U = subst_PTm (scons a0 VarPTm) P0 ->
-  funcomp (ren_PTm shift) (scons PNat Γ) ⊢ P0 ∈ PUniv i ->
-  funcomp (ren_PTm shift) (scons PNat Γ) ⊢ P0 ≡ P1 ∈ PUniv i ->
+  (cons PNat Γ) ⊢ P0 ∈ PUniv i ->
+  (cons PNat Γ) ⊢ P0 ≡ P1 ∈ PUniv i ->
   Γ ⊢ a0 ≡ a1 ∈ PNat ->
   Γ ⊢ b0 ≡ b1 ∈ subst_PTm (scons PZero VarPTm) P0 ->
-  funcomp (ren_PTm shift) (scons P0 (funcomp (ren_PTm shift) (scons PNat Γ))) ⊢ c0 ≡ c1 ∈ ren_PTm shift (subst_PTm (scons (PSuc (VarPTm var_zero)) (funcomp VarPTm shift) ) P0) ->
+  (cons P0 (cons PNat Γ)) ⊢ c0 ≡ c1 ∈ ren_PTm shift (subst_PTm (scons (PSuc (VarPTm var_zero)) (funcomp VarPTm shift) ) P0) ->
   Γ ⊢ PInd P0 a0 b0 c0 ≡ PInd P1 a1 b1 c1 ∈ U.
 Proof. move => ->. apply E_IndCong. Qed.
 
-Lemma T_Ind' s Γ P (a : PTm s) b c i U :
+Lemma T_Ind' Γ P (a : PTm) b c i U :
   U = subst_PTm (scons a VarPTm) P ->
-  funcomp (ren_PTm shift) (scons PNat Γ) ⊢ P ∈ PUniv i ->
+  cons PNat Γ ⊢ P ∈ PUniv i ->
   Γ ⊢ a ∈ PNat ->
   Γ ⊢ b ∈ subst_PTm (scons PZero VarPTm) P ->
-  funcomp (ren_PTm shift)(scons P (funcomp (ren_PTm shift) (scons PNat Γ))) ⊢ c ∈ ren_PTm shift (subst_PTm (scons (PSuc (VarPTm var_zero)) (funcomp VarPTm shift) ) P) ->
+  cons P (cons PNat Γ) ⊢ c ∈ ren_PTm shift (subst_PTm (scons (PSuc (VarPTm var_zero)) (funcomp VarPTm shift) ) P) ->
   Γ ⊢ PInd P a b c ∈ U.
 Proof. move =>->. apply T_Ind. Qed.
 
-Lemma T_Proj2' n Γ (a : PTm n) A B U :
+Lemma T_Proj2' Γ (a : PTm) A B U :
   U = subst_PTm (scons (PProj PL a) VarPTm) B ->
   Γ ⊢ a ∈ PBind PSig A B ->
   Γ ⊢ PProj PR a ∈ U.
 Proof. move => ->. apply T_Proj2. Qed.
 
-Lemma E_Proj2' n Γ i (a b : PTm n) A B U :
+Lemma E_Proj2' Γ i (a b : PTm) A B U :
   U = subst_PTm (scons (PProj PL a) VarPTm) B ->
   Γ ⊢ PBind PSig A B ∈ (PUniv i) ->
   Γ ⊢ a ≡ b ∈ PBind PSig A B ->
   Γ ⊢ PProj PR a ≡ PProj PR b ∈ U.
 Proof. move => ->. apply E_Proj2. Qed.
 
-Lemma E_Bind' n Γ i p (A0 A1 : PTm n) B0 B1 :
+Lemma E_Bind' Γ i p (A0 A1 : PTm) B0 B1 :
   Γ ⊢ A0 ∈ PUniv i ->
   Γ ⊢ A0 ≡ A1 ∈ PUniv i ->
-  funcomp (ren_PTm shift) (scons A0 Γ) ⊢ B0 ≡ B1 ∈ PUniv i ->
+  cons A0 Γ ⊢ B0 ≡ B1 ∈ PUniv i ->
   Γ ⊢ PBind p A0 B0 ≡ PBind p A1 B1 ∈ PUniv i.
 Proof. hauto lq:on use:E_Bind, wff_mutual. Qed.
 
-Lemma E_App' n Γ i (b0 b1 a0 a1 : PTm n) A B U :
+Lemma E_App' Γ i (b0 b1 a0 a1 : PTm) A B U :
   U = subst_PTm (scons a0 VarPTm) B ->
   Γ ⊢ PBind PPi A B ∈ (PUniv i) ->
   Γ ⊢ b0 ≡ b1 ∈ PBind PPi A B ->
@@ -120,16 +120,16 @@ Lemma E_App' n Γ i (b0 b1 a0 a1 : PTm n) A B U :
   Γ ⊢ PApp b0 a0 ≡ PApp b1 a1 ∈ U.
 Proof. move => ->. apply E_App. Qed.
 
-Lemma E_AppAbs' n Γ (a : PTm (S n)) b A B i u U :
+Lemma E_AppAbs' Γ (a : PTm) b A B i u U :
   u = subst_PTm (scons b VarPTm) a ->
   U = subst_PTm (scons b VarPTm ) B ->
   Γ ⊢ PBind PPi A B ∈ PUniv i ->
   Γ ⊢ b ∈ A ->
-  funcomp (ren_PTm shift) (scons A Γ) ⊢ a ∈ B ->
+  cons A Γ ⊢ a ∈ B ->
   Γ ⊢ PApp (PAbs a) b ≡ u ∈ U.
   move => -> ->. apply E_AppAbs. Qed.
 
-Lemma E_ProjPair2' n Γ (a b : PTm n) A B i U :
+Lemma E_ProjPair2' Γ (a b : PTm) A B i U :
   U = subst_PTm (scons a VarPTm) B ->
   Γ ⊢ PBind PSig A B ∈ (PUniv i) ->
   Γ ⊢ a ∈ A ->
@@ -137,14 +137,14 @@ Lemma E_ProjPair2' n Γ (a b : PTm n) A B i U :
   Γ ⊢ PProj PR (PPair a b) ≡ b ∈ U.
 Proof. move => ->. apply E_ProjPair2. Qed.
 
-Lemma E_AppEta' n Γ (b : PTm n) A B i u :
+Lemma E_AppEta' Γ (b : PTm ) A B i u :
   u = (PApp (ren_PTm shift b) (VarPTm var_zero)) ->
   Γ ⊢ PBind PPi A B ∈ (PUniv i) ->
   Γ ⊢ b ∈ PBind PPi A B ->
   Γ ⊢ PAbs u ≡ b ∈ PBind PPi A B.
 Proof. qauto l:on use:wff_mutual, E_AppEta. Qed.
 
-Lemma Su_Pi_Proj2' n Γ (a0 a1 A0 A1 : PTm n) B0 B1 U T :
+Lemma Su_Pi_Proj2' Γ (a0 a1 A0 A1 : PTm ) B0 B1 U T :
   U = subst_PTm (scons a0 VarPTm) B0 ->
   T = subst_PTm (scons a1 VarPTm) B1 ->
   Γ ⊢ PBind PPi A0 B0 ≲ PBind PPi A1 B1 ->
@@ -152,7 +152,7 @@ Lemma Su_Pi_Proj2' n Γ (a0 a1 A0 A1 : PTm n) B0 B1 U T :
   Γ ⊢ U ≲ T.
 Proof. move => -> ->. apply Su_Pi_Proj2. Qed.
 
-Lemma Su_Sig_Proj2' n Γ (a0 a1 A0 A1 : PTm n) B0 B1 U T :
+Lemma Su_Sig_Proj2' Γ (a0 a1 A0 A1 : PTm) B0 B1 U T :
   U = subst_PTm (scons a0 VarPTm) B0 ->
   T = subst_PTm (scons a1 VarPTm) B1 ->
   Γ ⊢ PBind PSig A0 B0 ≲ PBind PSig A1 B1 ->
@@ -160,64 +160,61 @@ Lemma Su_Sig_Proj2' n Γ (a0 a1 A0 A1 : PTm n) B0 B1 U T :
   Γ ⊢ U ≲ T.
 Proof. move => -> ->. apply Su_Sig_Proj2. Qed.
 
-Lemma E_IndZero' n Γ P i (b : PTm n) c U :
+Lemma E_IndZero' Γ P i (b : PTm) c U :
   U = subst_PTm (scons PZero VarPTm) P ->
-  funcomp (ren_PTm shift) (scons PNat Γ) ⊢ P ∈ PUniv i ->
+  cons PNat Γ ⊢ P ∈ PUniv i ->
   Γ ⊢ b ∈ subst_PTm (scons PZero VarPTm) P ->
-  funcomp (ren_PTm shift)(scons P (funcomp (ren_PTm shift) (scons PNat Γ))) ⊢ c ∈ ren_PTm shift (subst_PTm (scons (PSuc (VarPTm var_zero)) (funcomp VarPTm shift) ) P) ->
+  cons P (cons PNat Γ) ⊢ c ∈ ren_PTm shift (subst_PTm (scons (PSuc (VarPTm var_zero)) (funcomp VarPTm shift) ) P) ->
   Γ ⊢ PInd P PZero b c ≡ b ∈ U.
 Proof. move => ->. apply E_IndZero. Qed.
 
-Lemma Wff_Cons' n Γ (A : PTm n) i :
+Lemma Wff_Cons' Γ (A : PTm) i :
   Γ ⊢ A ∈ PUniv i ->
   (* -------------------------------- *)
-  ⊢ funcomp (ren_PTm shift) (scons A Γ).
+  ⊢ cons A Γ.
 Proof. hauto lq:on rew:off use:Wff_Cons, wff_mutual. Qed.
 
-Lemma E_IndSuc' s Γ P (a : PTm s) b c i u U :
+Lemma E_IndSuc' Γ P (a : PTm) b c i u U :
   u = subst_PTm (scons (PInd P a b c) (scons a VarPTm)) c ->
   U = subst_PTm (scons (PSuc a) VarPTm) P ->
-  funcomp (ren_PTm shift) (scons PNat Γ) ⊢ P ∈ PUniv i ->
+  cons PNat Γ ⊢ P ∈ PUniv i ->
   Γ ⊢ a ∈ PNat ->
   Γ ⊢ b ∈ subst_PTm (scons PZero VarPTm) P ->
-  funcomp (ren_PTm shift)(scons P (funcomp (ren_PTm shift) (scons PNat Γ))) ⊢ c ∈ ren_PTm shift (subst_PTm (scons (PSuc (VarPTm var_zero)) (funcomp VarPTm shift) ) P) ->
+  (cons P (cons PNat Γ)) ⊢ c ∈ ren_PTm shift (subst_PTm (scons (PSuc (VarPTm var_zero)) (funcomp VarPTm shift) ) P) ->
   Γ ⊢ PInd P (PSuc a) b c ≡ u ∈ U.
 Proof. move => ->->. apply E_IndSuc. Qed.
 
 Lemma renaming :
-  (forall n (Γ : fin n -> PTm n), ⊢ Γ -> True) /\
-  (forall n Γ (a A : PTm n), Γ ⊢ a ∈ A -> forall m Δ (ξ : fin n -> fin m), ⊢ Δ -> renaming_ok Δ Γ ξ ->
+  (forall Γ, ⊢ Γ -> True) /\
+  (forall Γ (a A : PTm), Γ ⊢ a ∈ A -> forall Δ (ξ : nat -> nat), ⊢ Δ -> renaming_ok Δ Γ ξ ->
      Δ ⊢ ren_PTm ξ a ∈ ren_PTm ξ A) /\
-  (forall n Γ (a b A : PTm n), Γ ⊢ a ≡ b ∈ A -> forall m Δ (ξ : fin n -> fin m), ⊢ Δ -> renaming_ok Δ Γ ξ ->
+  (forall Γ (a b A : PTm), Γ ⊢ a ≡ b ∈ A -> forall Δ (ξ : nat -> nat), ⊢ Δ -> renaming_ok Δ Γ ξ ->
      Δ ⊢ ren_PTm ξ a ≡ ren_PTm ξ b ∈ ren_PTm ξ A) /\
-  (forall n Γ (A B : PTm n), Γ ⊢ A ≲ B -> forall  m Δ (ξ : fin n -> fin m), ⊢ Δ -> renaming_ok Δ Γ ξ ->
+  (forall Γ (A B : PTm), Γ ⊢ A ≲ B -> forall  Δ (ξ : nat -> nat), ⊢ Δ -> renaming_ok Δ Γ ξ ->
     Δ ⊢ ren_PTm ξ A ≲ ren_PTm ξ B).
 Proof.
   apply wt_mutual => //=; eauto 3 with wt.
-  - move => n Γ i hΓ _ m Δ ξ hΔ hξ.
-    rewrite hξ.
-    by apply T_Var.
   - hauto lq:on rew:off ctrs:Wt, Wff  use:renaming_up.
-  - move => n Γ a A B i hP ihP ha iha m Δ ξ hΔ hξ.
+  - move => Γ a A B i hP ihP ha iha Δ ξ hΔ hξ.
     apply : T_Abs; eauto.
     move : ihP(hΔ) (hξ); repeat move/[apply]. move/Bind_Inv.
     hauto lq:on rew:off ctrs:Wff,Wt use:renaming_up.
   - move => *. apply : T_App'; eauto. by asimpl.
-  - move => n Γ a A b B i hA ihA hB ihB hS ihS m Δ ξ hξ hΔ.
+  - move => Γ a A b B i hA ihA hB ihB hS ihS Δ ξ hξ hΔ.
     eapply T_Pair' with (U := ren_PTm ξ (subst_PTm (scons a VarPTm) B));eauto. by asimpl.
-  - move => n Γ a A B ha iha m Δ ξ hΔ hξ. apply : T_Proj2'; eauto. by asimpl.
-  - move => s Γ P a b c i hP ihP ha iha hb ihb hc ihc m Δ ξ hΔ hξ.
+  - move => Γ a A B ha iha Δ ξ hΔ hξ. apply : T_Proj2'; eauto. by asimpl.
+  - move => Γ P a b c i hP ihP ha iha hb ihb hc ihc Δ ξ hΔ hξ.
     move => [:hP].
     apply : T_Ind'; eauto. by asimpl.
     abstract :hP. apply ihP. by eauto using Wff_Cons', T_Nat'.
     hauto l:on use:renaming_up.
     set x := subst_PTm _ _. have -> : x = ren_PTm ξ (subst_PTm (scons PZero VarPTm) P) by subst x; asimpl.
     by subst x; eauto.
-    set Ξ := funcomp _ _.
+    set Ξ := cons _ _.
     have  hΞ : ⊢ Ξ. subst Ξ.
     apply : Wff_Cons'; eauto. apply hP.
-    move /(_ _ Ξ (upRen_PTm_PTm (upRen_PTm_PTm ξ)) hΞ) : ihc.
-    set Ξ' := (funcomp _ _ : fin (S (S _)) -> _) .
+    move /(_ Ξ (upRen_PTm_PTm (upRen_PTm_PTm ξ)) hΞ) : ihc.
+    set Ξ' := (cons _ _) .
     have : renaming_ok Ξ Ξ' (upRen_PTm_PTm (upRen_PTm_PTm ξ)).
     by do 2 apply renaming_up.
     move /[swap] /[apply].
@@ -225,31 +222,33 @@ Proof.
   - hauto lq:on ctrs:Wt,LEq.
   - hauto lq:on ctrs:Eq.
   - hauto lq:on rew:off use:E_Bind', Wff_Cons, renaming_up.
-  - move => n Γ a b A B i hPi ihPi ha iha m Δ ξ hΔ hξ.
+  - move => Γ a b A B i hPi ihPi ha iha Δ ξ hΔ hξ.
     move : ihPi (hΔ) (hξ). repeat move/[apply].
     move => /Bind_Inv [j][h0][h1]h2.
     have ? : Δ ⊢ PBind PPi (ren_PTm ξ A) (ren_PTm (upRen_PTm_PTm ξ) B) ∈ PUniv j by qauto l:on ctrs:Wt.
     move {hPi}.
     apply : E_Abs; eauto. qauto l:on ctrs:Wff use:renaming_up.
   - move => *. apply : E_App'; eauto. by asimpl.
-  - move => n Γ a0 a1 b0 b1 A B i hA ihA ha iha hb ihb m Δ ξ hΔ hξ.
+  - move => Γ a0 a1 b0 b1 A B i hA ihA ha iha hb ihb Δ ξ hΔ hξ.
     apply : E_Pair; eauto.
     move : ihb hΔ hξ. repeat move/[apply].
     by asimpl.
   - move => *. apply : E_Proj2'; eauto. by asimpl.
-  - move => n Γ P0 P1 a0 a1 b0 b1 c0 c1 i hP0 ihP0 hP ihP ha iha hb ihb hc ihc.
-    move => m Δ ξ hΔ hξ [:hP'].
-    apply E_IndCong' with (i := i).
+  - move => Γ P0 P1 a0 a1 b0 b1 c0 c1 i hP0 ihP0 hP ihP ha iha hb ihb hc ihc.
+    move => Δ ξ hΔ hξ [:hP' hren].
+    apply E_IndCong' with (i := i); eauto with wt.
     by asimpl.
+    apply ihP0.
     abstract : hP'.
     qauto l:on use:renaming_up, Wff_Cons', T_Nat'.
+    abstract : hren.
     qauto l:on use:renaming_up, Wff_Cons', T_Nat'.
-    by eauto with wt.
+    apply ihP; eauto with wt.
     move : ihb (hΔ) (hξ); do! move/[apply]. by asimpl.
-    set Ξ := funcomp _ _.
+    set Ξ := cons _ _.
     have hΞ : ⊢ Ξ.
-    subst Ξ. apply :Wff_Cons'; eauto. apply hP'.
-    move /(_ _ Ξ  (upRen_PTm_PTm (upRen_PTm_PTm ξ)) hΞ) : ihc.
+    subst Ξ. apply :Wff_Cons'; eauto.
+    move /(_ Ξ  (upRen_PTm_PTm (upRen_PTm_PTm ξ)) hΞ) : ihc.
     move /(_ ltac:(qauto l:on use:renaming_up)).
     suff : ren_PTm (upRen_PTm_PTm (upRen_PTm_PTm ξ))
       (ren_PTm shift
@@ -259,31 +258,33 @@ Proof.
          (ren_PTm (upRen_PTm_PTm ξ) P0)) by scongruence.
     by asimpl.
   - qauto l:on ctrs:Eq, LEq.
-  - move => n Γ a b A B i hP ihP hb ihb ha iha m Δ ξ hΔ hξ.
+  - move => Γ a b A B i hP ihP hb ihb ha iha Δ ξ hΔ hξ.
     move : ihP (hξ) (hΔ). repeat move/[apply].
     move /Bind_Inv.
     move => [j][h0][h1]h2.
     have ? : Δ ⊢ PBind PPi (ren_PTm ξ A) (ren_PTm (upRen_PTm_PTm ξ) B) ∈ PUniv j by qauto l:on ctrs:Wt.
     apply : E_AppAbs'; eauto. by asimpl. by asimpl.
     hauto lq:on ctrs:Wff use:renaming_up.
-  - move => n Γ a b A B i hP ihP ha iha hb ihb m Δ ξ hΔ hξ.
+  - move => Γ a b A B i hP ihP ha iha hb ihb Δ ξ hΔ hξ.
     move : {hP} ihP (hξ) (hΔ). repeat move/[apply].
     move /Bind_Inv => [i0][h0][h1]h2.
     have ? : Δ ⊢ PBind PSig (ren_PTm ξ A) (ren_PTm (upRen_PTm_PTm ξ) B) ∈ PUniv i0 by qauto l:on ctrs:Wt.
     apply : E_ProjPair1; eauto.
     move : ihb hξ hΔ. repeat move/[apply]. by asimpl.
-  - move => n Γ a b A B i hP ihP ha iha hb ihb m Δ ξ hΔ hξ.
+  - move => Γ a b A B i hP ihP ha iha hb ihb Δ ξ hΔ hξ.
     apply : E_ProjPair2'; eauto. by asimpl.
     move : ihb hξ hΔ; repeat move/[apply]. by asimpl.
-  - move => n Γ P i b c hP ihP hb ihb hc ihc m Δ ξ hΔ hξ.
+  - move => Γ P i b c hP ihP hb ihb hc ihc Δ ξ hΔ hξ.
     apply E_IndZero' with (i := i); eauto. by asimpl.
-    qauto l:on use:Wff_Cons', T_Nat', renaming_up.
-    move  /(_ m Δ ξ hΔ) : ihb.
+    sauto lq:on use:Wff_Cons', T_Nat', renaming_up.
+    move  /(_ Δ ξ hΔ) : ihb.
     asimpl. by apply.
-    set Ξ := funcomp _ _.
-    have hΞ : ⊢ Ξ by  qauto l:on use:Wff_Cons', T_Nat', renaming_up.
-    move /(_ _ Ξ  (upRen_PTm_PTm (upRen_PTm_PTm ξ)) hΞ) : ihc.
-    move /(_ ltac:(qauto l:on use:renaming_up)).
+    set Ξ := cons _ _.
+    have hΞ : ⊢ Ξ by  sauto lq:on use:Wff_Cons', T_Nat', renaming_up.
+    move /(_ Ξ  (upRen_PTm_PTm (upRen_PTm_PTm ξ)) hΞ) : ihc.
+    set p := renaming_ok _ _ _.
+    have : p. by do 2 apply renaming_up.
+    move => /[swap]/[apply].
     suff : ren_PTm (upRen_PTm_PTm (upRen_PTm_PTm ξ))
       (ren_PTm shift
          (subst_PTm
@@ -291,15 +292,15 @@ Proof.
       (subst_PTm (scons (PSuc (VarPTm var_zero)) (funcomp VarPTm shift))
          (ren_PTm (upRen_PTm_PTm ξ) P)) by scongruence.
     by asimpl.
-  - move => n Γ P a b c i hP ihP ha iha hb ihb hc ihc m Δ ξ hΔ hξ.
+  - move => Γ P a b c i hP ihP ha iha hb ihb hc ihc Δ ξ hΔ hξ.
     apply E_IndSuc' with (i := i). by asimpl. by asimpl.
-    qauto l:on use:Wff_Cons', T_Nat', renaming_up.
+    sauto lq:on use:Wff_Cons', T_Nat', renaming_up.
     by eauto with wt.
-    move  /(_ m Δ ξ hΔ) : ihb. asimpl. by apply.
-    set Ξ := funcomp _ _.
-    have hΞ : ⊢ Ξ by  qauto l:on use:Wff_Cons', T_Nat', renaming_up.
-    move /(_ _ Ξ  (upRen_PTm_PTm (upRen_PTm_PTm ξ)) hΞ) : ihc.
-    move /(_ ltac:(qauto l:on use:renaming_up)).
+    move  /(_ Δ ξ hΔ) : ihb. asimpl. by apply.
+    set Ξ := cons _ _.
+    have hΞ : ⊢ Ξ by  sauto lq:on use:Wff_Cons', T_Nat', renaming_up.
+    move /(_ Ξ  (upRen_PTm_PTm (upRen_PTm_PTm ξ)) hΞ) : ihc.
+    move /(_ ltac:(by eauto using renaming_up)).
     by asimpl.
   - move => *.
     apply : E_AppEta'; eauto. by asimpl.
@@ -315,94 +316,94 @@ Proof.
   - move => *. apply : Su_Sig_Proj2'; eauto; by asimpl.
 Qed.
 
-Definition morphing_ok {n m} Δ Γ (ρ : fin n -> PTm m) :=
-  forall i, Δ ⊢ ρ i ∈ subst_PTm ρ (Γ i).
+Definition morphing_ok Δ Γ (ρ : nat -> PTm) :=
+  forall i A, lookup i Γ A -> Δ ⊢ ρ i ∈ subst_PTm ρ A.
 
-Lemma morphing_ren n m p Ξ Δ Γ
-  (ρ : fin n -> PTm m) (ξ : fin m -> fin p) :
+Lemma morphing_ren Ξ Δ Γ
+  (ρ : nat -> PTm) (ξ : nat -> nat) :
   ⊢ Ξ ->
   renaming_ok Ξ Δ ξ -> morphing_ok Δ Γ ρ ->
   morphing_ok Ξ Γ (funcomp (ren_PTm ξ) ρ).
 Proof.
-  move => hΞ hξ hρ.
-  move => i.
+  move => hΞ hξ hρ i A.
   rewrite {1}/funcomp.
   have -> :
-    subst_PTm (funcomp (ren_PTm ξ) ρ) (Γ i) =
-    ren_PTm ξ (subst_PTm ρ (Γ i)) by asimpl.
-  eapply renaming; eauto.
+    subst_PTm (funcomp (ren_PTm ξ) ρ) A =
+    ren_PTm ξ (subst_PTm ρ A) by asimpl.
+  move => ?.  eapply renaming; eauto.
 Qed.
 
-Lemma morphing_ext n m Δ Γ (ρ : fin n -> PTm m) (a : PTm m) (A : PTm n)  :
+Lemma morphing_ext Δ Γ (ρ : nat -> PTm) (a : PTm) (A : PTm)  :
   morphing_ok Δ Γ ρ ->
   Δ ⊢ a ∈ subst_PTm ρ A ->
   morphing_ok
-  Δ (funcomp (ren_PTm shift) (scons A Γ)) (scons a ρ).
+    Δ (cons A Γ) (scons a ρ).
 Proof.
-  move => h ha i. destruct i as [i|]; by asimpl.
+  move => h ha i B.
+  elim /lookup_inv => //=_.
+  - move => A0 Γ0 ? [*]. subst.
+    by asimpl.
+  - move => i0 Γ0 A0 B0 h0 ? [*]. subst.
+    asimpl. by apply h.
 Qed.
 
-Lemma T_Var' n Γ (i : fin n) U :
-  U = Γ i ->
-  ⊢ Γ ->
-  Γ ⊢ VarPTm i ∈ U.
-Proof. move => ->. apply T_Var. Qed.
-
-Lemma renaming_wt : forall n Γ (a A : PTm n), Γ ⊢ a ∈ A -> forall m Δ (ξ : fin n -> fin m), ⊢ Δ -> renaming_ok Δ Γ ξ -> Δ ⊢ ren_PTm ξ a ∈ ren_PTm ξ A.
+Lemma renaming_wt : forall Γ (a A : PTm), Γ ⊢ a ∈ A -> forall Δ (ξ : nat -> nat), ⊢ Δ -> renaming_ok Δ Γ ξ -> Δ ⊢ ren_PTm ξ a ∈ ren_PTm ξ A.
 Proof. sfirstorder use:renaming. Qed.
 
-Lemma renaming_wt' : forall n m Δ Γ a A (ξ : fin n -> fin m) u U,
+Lemma renaming_wt' : forall Δ Γ a A (ξ : nat -> nat) u U,
     u = ren_PTm ξ a -> U = ren_PTm ξ A ->
     Γ ⊢ a ∈ A -> ⊢ Δ ->
     renaming_ok Δ Γ ξ -> Δ ⊢ u ∈ U.
 Proof. hauto use:renaming_wt. Qed.
 
-Lemma morphing_up n m Γ Δ (ρ : fin n -> PTm m) (A : PTm n) k :
+Lemma morphing_up Γ Δ (ρ : nat -> PTm) (A : PTm) k :
   morphing_ok Γ Δ ρ ->
   Γ ⊢ subst_PTm ρ A ∈ PUniv k ->
-  morphing_ok (funcomp (ren_PTm shift) (scons (subst_PTm ρ A) Γ)) (funcomp (ren_PTm shift) (scons A Δ)) (up_PTm_PTm ρ).
+  morphing_ok (cons (subst_PTm ρ A) Γ) (cons A Δ) (up_PTm_PTm ρ).
 Proof.
   move => h h1 [:hp]. apply morphing_ext.
   rewrite /morphing_ok.
-  move => i.
-  rewrite {2}/funcomp.
-  apply : renaming_wt'; eauto. by asimpl.
+  move => i A0 hA0.
+  apply : renaming_wt'; last by apply renaming_shift.
+  rewrite /funcomp. reflexivity.
+  2 : { eauto. }
+  by asimpl.
   abstract : hp. qauto l:on ctrs:Wff use:wff_mutual.
-  eauto using renaming_shift.
-  apply : T_Var';eauto. rewrite /funcomp. by asimpl.
+  apply : T_Var;eauto. apply here'. by asimpl.
 Qed.
 
-Lemma weakening_wt : forall n Γ (a A B : PTm n) i,
+Lemma weakening_wt : forall Γ (a A B : PTm) i,
     Γ ⊢ B ∈ PUniv i ->
     Γ ⊢ a ∈ A ->
-    funcomp (ren_PTm shift) (scons B Γ) ⊢ ren_PTm shift a ∈ ren_PTm shift A.
+    cons B Γ ⊢ ren_PTm shift a ∈ ren_PTm shift A.
 Proof.
-  move => n Γ a A B i hB ha.
+  move => Γ a A B i hB ha.
   apply : renaming_wt'; eauto.
   apply : Wff_Cons'; eauto.
   apply : renaming_shift; eauto.
 Qed.
 
-Lemma weakening_wt' : forall n Γ (a A B : PTm n) i U u,
+Lemma weakening_wt' : forall Γ (a A B : PTm) i U u,
     u = ren_PTm shift a ->
     U = ren_PTm shift A ->
     Γ ⊢ B ∈ PUniv i ->
     Γ ⊢ a ∈ A ->
-    funcomp (ren_PTm shift) (scons B Γ) ⊢ u ∈ U.
+    cons B Γ ⊢ u ∈ U.
 Proof. move => > -> ->. apply weakening_wt. Qed.
 
 Lemma morphing :
-  (forall n (Γ : fin n -> PTm n), ⊢ Γ -> True) /\
-  (forall n Γ (a A : PTm n), Γ ⊢ a ∈ A -> forall m Δ (ρ : fin n -> PTm m), ⊢ Δ -> morphing_ok Δ Γ ρ ->
+  (forall Γ, ⊢ Γ -> True) /\
+    (forall Γ a A, Γ ⊢ a ∈ A -> forall Δ ρ, ⊢ Δ -> morphing_ok Δ Γ ρ ->
      Δ ⊢ subst_PTm ρ a ∈ subst_PTm ρ A) /\
-  (forall n Γ (a b A : PTm n), Γ ⊢ a ≡ b ∈ A -> forall m Δ (ρ : fin n -> PTm m), ⊢ Δ -> morphing_ok Δ Γ ρ ->
+    (forall Γ a b A, Γ ⊢ a ≡ b ∈ A -> forall Δ ρ, ⊢ Δ -> morphing_ok Δ Γ ρ ->
      Δ ⊢ subst_PTm ρ a ≡ subst_PTm ρ b ∈ subst_PTm ρ A) /\
-  (forall n Γ (A B : PTm n), Γ ⊢ A ≲ B -> forall  m Δ (ρ : fin n -> PTm m), ⊢ Δ -> morphing_ok Δ Γ ρ ->
+    (forall Γ A B, Γ ⊢ A ≲ B -> forall Δ ρ, ⊢ Δ -> morphing_ok Δ Γ ρ ->
     Δ ⊢ subst_PTm ρ A ≲ subst_PTm ρ B).
 Proof.
   apply wt_mutual => //=.
+  - hauto l:on unfold:morphing_ok.
   - hauto lq:on use:morphing_up, Wff_Cons', T_Bind.
-  - move => n Γ a A B i hP ihP ha iha m Δ ρ hΔ hρ.
+  - move => Γ a A B i hP ihP ha iha Δ ρ hΔ hρ.
     move : ihP (hΔ) (hρ); repeat move/[apply].
     move /Bind_Inv => [j][h0][h1]h2. move {hP}.
     have ? : Δ ⊢ PBind PPi (subst_PTm ρ A) (subst_PTm (up_PTm_PTm ρ) B) ∈ PUniv i by hauto lq:on ctrs:Wt.
@@ -411,7 +412,7 @@ Proof.
     hauto lq:on use:Wff_Cons', Bind_Inv.
     apply : morphing_up; eauto.
   - move => *; apply : T_App'; eauto; by asimpl.
-  - move => n Γ a A b B i hA ihA hB ihB hS ihS m Δ ρ hρ hΔ.
+  - move => Γ a A b B i hA ihA hB ihB hS ihS Δ ρ hρ hΔ.
     eapply T_Pair' with (U := subst_PTm ρ (subst_PTm (scons a VarPTm) B));eauto. by asimpl.
   - hauto lq:on use:T_Proj1.
   - move => *. apply : T_Proj2'; eauto. by asimpl.
@@ -419,9 +420,8 @@ Proof.
   - qauto l:on ctrs:Wt.
   - qauto l:on ctrs:Wt.
   - qauto l:on ctrs:Wt.
-  - move => s Γ P a b c i hP ihP ha iha hb ihb hc ihc m Δ ξ hΔ hξ.
-    have  hξ' : morphing_ok (funcomp (ren_PTm shift) (scons PNat Δ))
-    (funcomp (ren_PTm shift) (scons PNat Γ)) (up_PTm_PTm ξ).
+  - move => Γ P a b c i hP ihP ha iha hb ihb hc ihc Δ ξ hΔ hξ.
+    have  hξ' : morphing_ok (cons PNat Δ) (cons PNat Γ) (up_PTm_PTm ξ).
     move /morphing_up : hξ.  move /(_ PNat 0).
     apply. by apply T_Nat.
     move => [:hP].
@@ -430,11 +430,11 @@ Proof.
     move /morphing_up : hξ.  move /(_ PNat 0).
     apply. by apply T_Nat.
     move : ihb hξ hΔ; do!move/[apply]. by asimpl.
-    set Ξ := funcomp _ _.
+    set Ξ := cons _ _.
     have  hΞ : ⊢ Ξ. subst Ξ.
     apply : Wff_Cons'; eauto. apply hP.
-    move /(_ _ Ξ (up_PTm_PTm (up_PTm_PTm ξ)) hΞ) : ihc.
-    set Ξ' := (funcomp _ _ : fin (S (S _)) -> _) .
+    move /(_ Ξ (up_PTm_PTm (up_PTm_PTm ξ)) hΞ) : ihc.
+    set Ξ' := (cons _ _) .
     have : morphing_ok Ξ Ξ' (up_PTm_PTm (up_PTm_PTm ξ)).
     eapply morphing_up; eauto. apply hP.
     move /[swap]/[apply].
@@ -447,23 +447,23 @@ Proof.
   - hauto lq:on ctrs:Eq.
   - hauto lq:on ctrs:Eq.
   - hauto lq:on rew:off use:E_Bind', Wff_Cons, morphing_up.
-  - move => n Γ a b A B i hPi ihPi ha iha m Δ ρ hΔ hρ.
+  - move => Γ a b A B i hPi ihPi ha iha Δ ρ hΔ hρ.
     move : ihPi (hΔ) (hρ). repeat move/[apply].
     move => /Bind_Inv [j][h0][h1]h2.
     have ? : Δ ⊢ PBind PPi (subst_PTm ρ A) (subst_PTm (up_PTm_PTm ρ) B) ∈ PUniv j by qauto l:on ctrs:Wt.
     move {hPi}.
     apply : E_Abs; eauto. qauto l:on ctrs:Wff use:morphing_up.
   - move => *. apply : E_App'; eauto. by asimpl.
-  - move => n Γ a0 a1 b0 b1 A B i hA ihA ha iha hb ihb m Δ ρ hΔ hρ.
+  - move => Γ a0 a1 b0 b1 A B i hA ihA ha iha hb ihb Δ ρ hΔ hρ.
     apply : E_Pair; eauto.
     move : ihb hΔ hρ. repeat move/[apply].
     by asimpl.
   - hauto q:on ctrs:Eq.
   - move => *. apply : E_Proj2'; eauto. by asimpl.
-  - move => n Γ P0 P1 a0 a1 b0 b1 c0 c1 i hP0 ihP0 hP ihP ha iha hb ihb hc ihc.
-    move => m Δ ξ hΔ hξ.
-    have  hξ' : morphing_ok (funcomp (ren_PTm shift) (scons PNat Δ))
-                  (funcomp (ren_PTm shift) (scons PNat Γ)) (up_PTm_PTm ξ).
+  - move => Γ P0 P1 a0 a1 b0 b1 c0 c1 i hP0 ihP0 hP ihP ha iha hb ihb hc ihc.
+    move => Δ ξ hΔ hξ.
+    have  hξ' : morphing_ok (cons PNat Δ)
+                   (cons PNat Γ) (up_PTm_PTm ξ).
     move /morphing_up : hξ.  move /(_ PNat 0).
     apply. by apply T_Nat.
     move => [:hP'].
@@ -474,56 +474,54 @@ Proof.
     qauto l:on use:renaming_up, Wff_Cons', T_Nat'.
     by eauto with wt.
     move : ihb (hΔ) (hξ); do! move/[apply]. by asimpl.
-    set Ξ := funcomp _ _.
+    set Ξ := cons _ _.
     have hΞ : ⊢ Ξ.
     subst Ξ. apply :Wff_Cons'; eauto. apply hP'.
-    move /(_ _ Ξ  (up_PTm_PTm (up_PTm_PTm ξ)) hΞ) : ihc.
+    move /(_ Ξ  (up_PTm_PTm (up_PTm_PTm ξ)) hΞ) : ihc.
     move /(_ ltac:(qauto l:on use:morphing_up)).
     asimpl. substify. by asimpl.
   - eauto with wt.
   - qauto l:on ctrs:Eq, LEq.
-  - move => n Γ a b A B i hP ihP hb ihb ha iha m Δ ρ hΔ hρ.
+  - move => Γ a b A B i hP ihP hb ihb ha iha Δ ρ hΔ hρ.
     move : ihP (hρ) (hΔ). repeat move/[apply].
     move /Bind_Inv.
     move => [j][h0][h1]h2.
     have ? : Δ ⊢ PBind PPi (subst_PTm ρ A) (subst_PTm (up_PTm_PTm ρ) B) ∈ PUniv j by qauto l:on ctrs:Wt.
     apply : E_AppAbs'; eauto. by asimpl. by asimpl.
     hauto lq:on ctrs:Wff use:morphing_up.
-  - move => n Γ a b A B i hP ihP ha iha hb ihb m Δ ρ hΔ hρ.
+  - move => Γ a b A B i hP ihP ha iha hb ihb Δ ρ hΔ hρ.
     move : {hP} ihP (hρ) (hΔ). repeat move/[apply].
     move /Bind_Inv => [i0][h0][h1]h2.
     have ? : Δ ⊢ PBind PSig (subst_PTm ρ A) (subst_PTm (up_PTm_PTm ρ) B) ∈ PUniv i0 by qauto l:on ctrs:Wt.
     apply : E_ProjPair1; eauto.
     move : ihb hρ hΔ. repeat move/[apply]. by asimpl.
-  - move => n Γ a b A B i hP ihP ha iha hb ihb m Δ ρ hΔ hρ.
+  - move => Γ a b A B i hP ihP ha iha hb ihb Δ ρ hΔ hρ.
     apply : E_ProjPair2'; eauto. by asimpl.
     move : ihb hρ hΔ; repeat move/[apply]. by asimpl.
-  - move => n Γ P i b c hP ihP hb ihb hc ihc m Δ ξ hΔ hξ.
-    have  hξ' : morphing_ok (funcomp (ren_PTm shift) (scons PNat Δ))
-                  (funcomp (ren_PTm shift) (scons PNat Γ)) (up_PTm_PTm ξ).
+  - move => Γ P i b c hP ihP hb ihb hc ihc Δ ξ hΔ hξ.
+    have  hξ' : morphing_ok (cons PNat Δ)(cons PNat Γ) (up_PTm_PTm ξ).
     move /morphing_up : hξ.  move /(_ PNat 0).
     apply. by apply T_Nat.
     apply E_IndZero' with (i := i); eauto. by asimpl.
     qauto l:on use:Wff_Cons', T_Nat', renaming_up.
-    move  /(_ m Δ ξ hΔ) : ihb.
+    move  /(_ Δ ξ hΔ) : ihb.
     asimpl. by apply.
-    set Ξ := funcomp _ _.
+    set Ξ := cons _ _.
     have hΞ : ⊢ Ξ by  qauto l:on use:Wff_Cons', T_Nat', renaming_up.
-    move /(_ _ Ξ  (up_PTm_PTm (up_PTm_PTm ξ)) hΞ) : ihc.
+    move /(_ Ξ  (up_PTm_PTm (up_PTm_PTm ξ)) hΞ) : ihc.
     move /(_ ltac:(sauto lq:on use:morphing_up)).
     asimpl. substify. by asimpl.
-  - move => n Γ P a b c i hP ihP ha iha hb ihb hc ihc m Δ ξ hΔ hξ.
-    have  hξ' : morphing_ok (funcomp (ren_PTm shift) (scons PNat Δ))
-                  (funcomp (ren_PTm shift) (scons PNat Γ)) (up_PTm_PTm ξ).
+  - move => Γ P a b c i hP ihP ha iha hb ihb hc ihc Δ ξ hΔ hξ.
+    have  hξ' : morphing_ok (cons PNat Δ) (cons PNat Γ) (up_PTm_PTm ξ).
     move /morphing_up : hξ.  move /(_ PNat 0).
     apply. by apply T_Nat'.
     apply E_IndSuc' with (i := i). by asimpl. by asimpl.
     qauto l:on use:Wff_Cons', T_Nat', renaming_up.
     by eauto with wt.
-    move  /(_ m Δ ξ hΔ) : ihb. asimpl. by apply.
-    set Ξ := funcomp _ _.
+    move  /(_ Δ ξ hΔ) : ihb. asimpl. by apply.
+    set Ξ := cons _ _.
     have hΞ : ⊢ Ξ by  qauto l:on use:Wff_Cons', T_Nat', renaming_up.
-    move /(_ _ Ξ  (up_PTm_PTm (up_PTm_PTm ξ)) hΞ) : ihc.
+    move /(_ Ξ  (up_PTm_PTm (up_PTm_PTm ξ)) hΞ) : ihc.
     move /(_ ltac:(sauto l:on use:morphing_up)).
     asimpl. substify. by asimpl.
   - move => *.
@@ -540,40 +538,39 @@ Proof.
   - move => *. apply : Su_Sig_Proj2'; eauto; by asimpl.
 Qed.
 
-Lemma morphing_wt : forall n Γ (a A : PTm n), Γ ⊢ a ∈ A -> forall m Δ (ρ : fin n -> PTm m), ⊢ Δ -> morphing_ok Δ Γ ρ -> Δ ⊢ subst_PTm ρ a ∈ subst_PTm ρ A.
+Lemma morphing_wt : forall Γ (a A : PTm ), Γ ⊢ a ∈ A -> forall Δ (ρ : nat -> PTm), ⊢ Δ -> morphing_ok Δ Γ ρ -> Δ ⊢ subst_PTm ρ a ∈ subst_PTm ρ A.
 Proof. sfirstorder use:morphing. Qed.
 
-Lemma morphing_wt' : forall n m Δ Γ a A (ρ : fin n -> PTm m) u U,
+Lemma morphing_wt' : forall Δ Γ a A (ρ : nat -> PTm) u U,
     u = subst_PTm ρ a -> U = subst_PTm ρ A ->
     Γ ⊢ a ∈ A -> ⊢ Δ ->
     morphing_ok Δ Γ ρ -> Δ ⊢ u ∈ U.
 Proof. hauto use:morphing_wt. Qed.
 
-Lemma morphing_id : forall n (Γ : fin n -> PTm n), ⊢ Γ -> morphing_ok Γ Γ VarPTm.
+Lemma morphing_id : forall Γ, ⊢ Γ -> morphing_ok Γ Γ VarPTm.
 Proof.
-  move => n Γ hΓ.
-  rewrite /morphing_ok.
-  move => i. asimpl. by apply T_Var.
+  rewrite /morphing_ok => Γ hΓ i. asimpl.
+  eauto using T_Var.
 Qed.
 
-Lemma substing_wt : forall n Γ (a : PTm (S n)) (b A : PTm n) B,
-    funcomp (ren_PTm shift) (scons A Γ) ⊢ a ∈ B ->
+Lemma substing_wt : forall Γ (a : PTm) (b A : PTm) B,
+    (cons A Γ) ⊢ a ∈ B ->
     Γ ⊢ b ∈ A ->
     Γ ⊢ subst_PTm (scons b VarPTm) a ∈ subst_PTm (scons b VarPTm) B.
 Proof.
-  move => n Γ a b A B ha hb [:hΓ]. apply : morphing_wt; eauto.
+  move => Γ a b A B ha hb [:hΓ]. apply : morphing_wt; eauto.
   abstract : hΓ. sfirstorder use:wff_mutual.
   apply morphing_ext; last by asimpl.
   by apply morphing_id.
 Qed.
 
 (* Could generalize to all equal contexts *)
-Lemma ctx_eq_subst_one n (A0 A1 : PTm n) i j Γ a A :
-  funcomp (ren_PTm shift) (scons A0 Γ) ⊢ a ∈ A ->
+Lemma ctx_eq_subst_one (A0 A1 : PTm) i j Γ a A :
+  (cons A0 Γ) ⊢ a ∈ A ->
   Γ ⊢ A0 ∈ PUniv i ->
   Γ ⊢ A1 ∈ PUniv j ->
   Γ ⊢ A1 ≲ A0 ->
-  funcomp (ren_PTm shift) (scons A1 Γ) ⊢ a ∈ A.
+  (cons A1 Γ) ⊢ a ∈ A.
 Proof.
   move => h0 h1 h2 h3.
   replace a with (subst_PTm VarPTm a); last by asimpl.
@@ -581,22 +578,23 @@ Proof.
   have ? : ⊢ Γ by sfirstorder use:wff_mutual.
   apply : morphing_wt; eauto.
   apply : Wff_Cons'; eauto.
-  move => k. destruct k as [k|].
-  - asimpl.
-    eapply weakening_wt' with (a := VarPTm k);eauto using T_Var.
+  move => k A2. elim/lookup_inv => //=_; cycle 1.
+  - move => i0 Γ0 A3 B hi ? [*]. subst.
+    asimpl.
+    eapply weakening_wt' with (a := VarPTm i0);eauto using T_Var.
     by substify.
-  - move => [:hΓ'].
+  - move => A3 Γ0 ? [*]. subst.
+    move => [:hΓ'].
     apply : T_Conv.
     apply T_Var.
     abstract : hΓ'.
-    eauto using Wff_Cons'.
-    rewrite /funcomp. asimpl. substify. asimpl.
-    renamify.
+    eauto using Wff_Cons'. apply here.
+    asimpl. renamify.
     eapply renaming; eauto.
     apply : renaming_shift; eauto.
 Qed.
 
-Lemma bind_inst n Γ p (A : PTm n) B i a0 a1 :
+Lemma bind_inst Γ p (A : PTm) B i a0 a1 :
   Γ ⊢ PBind p A B ∈ PUniv i ->
   Γ ⊢ a0 ≡ a1 ∈ A ->
   Γ ⊢ subst_PTm (scons a0 VarPTm) B ≲ subst_PTm (scons a1 VarPTm) B.
@@ -606,7 +604,7 @@ Proof.
   case : p h => //=; hauto l:on use:Su_Pi_Proj2, Su_Sig_Proj2.
 Qed.
 
-Lemma Cumulativity n Γ (a : PTm n) i j :
+Lemma Cumulativity Γ (a : PTm ) i j :
   i <= j ->
   Γ ⊢ a ∈ PUniv i ->
   Γ ⊢ a ∈ PUniv j.
@@ -616,9 +614,9 @@ Proof.
   sfirstorder use:wff_mutual.
 Qed.
 
-Lemma T_Bind' n Γ i j p (A : PTm n) (B : PTm (S n)) :
+Lemma T_Bind' Γ i j p (A : PTm ) (B : PTm) :
   Γ ⊢ A ∈ PUniv i ->
-  funcomp (ren_PTm shift) (scons A Γ) ⊢ B ∈ PUniv j ->
+  (cons A Γ) ⊢ B ∈ PUniv j ->
   Γ ⊢ PBind p A B ∈ PUniv (max i j).
 Proof.
   move => h0 h1.
@@ -629,47 +627,48 @@ Qed.
 Hint Resolve T_Bind' : wt.
 
 Lemma regularity :
-  (forall n (Γ : fin n -> PTm n), ⊢ Γ -> forall i, exists j, Γ ⊢ Γ i ∈ PUniv j) /\
-  (forall n Γ (a A : PTm n), Γ ⊢ a ∈ A -> exists i, Γ ⊢ A ∈ PUniv i)  /\
-  (forall n Γ (a b A : PTm n), Γ ⊢ a ≡ b ∈ A -> Γ ⊢ a ∈ A /\ Γ ⊢ b ∈ A /\ exists i, Γ ⊢ A ∈ PUniv i) /\
-  (forall n Γ (A B : PTm n), Γ ⊢ A ≲ B -> exists i, Γ ⊢ A ∈ PUniv i /\ Γ ⊢ B ∈ PUniv i).
+  (forall Γ, ⊢ Γ -> forall i A, lookup i Γ A -> exists j, Γ ⊢ A ∈ PUniv j) /\
+    (forall Γ a A, Γ ⊢ a ∈ A -> exists i, Γ ⊢ A ∈ PUniv i)  /\
+    (forall Γ a b A, Γ ⊢ a ≡ b ∈ A -> Γ ⊢ a ∈ A /\ Γ ⊢ b ∈ A /\ exists i, Γ ⊢ A ∈ PUniv i) /\
+    (forall Γ A B, Γ ⊢ A ≲ B -> exists i, Γ ⊢ A ∈ PUniv i /\ Γ ⊢ B ∈ PUniv i).
 Proof.
   apply wt_mutual => //=; eauto with wt.
-  - move => n Γ A i hΓ ihΓ hA _ j.
-    destruct j as [j|].
-    have := ihΓ j.
-    move => [j0 hj].
-    exists j0. apply : renaming_wt' => //=; eauto using renaming_shift.
-    reflexivity. econstructor; eauto.
-    exists i. rewrite {2}/funcomp. simpl.
-    apply : renaming_wt'; eauto. reflexivity.
-    econstructor; eauto.
-    apply : renaming_shift; eauto.
-  - move => n Γ b a A B hb [i ihb] ha [j iha].
+  - move => i A. elim/lookup_inv => //=_.
+  - move => Γ A i hΓ ihΓ hA _ j A0.
+    elim /lookup_inv => //=_; cycle 1.
+    + move => i0 Γ0 A1 B + ? [*]. subst.
+      move : ihΓ => /[apply]. move => [j hA1].
+      exists j. apply : renaming_wt' => //=; eauto using renaming_shift. done.
+      apply : Wff_Cons'; eauto.
+    + move => A1 Γ0 ? [*]. subst.
+      exists i. apply : renaming_wt'; eauto. reflexivity.
+      econstructor; eauto.
+      apply : renaming_shift; eauto.
+  - move => Γ b a A B hb [i ihb] ha [j iha].
     move /Bind_Inv : ihb => [k][h0][h1]h2.
     move : substing_wt ha h1; repeat move/[apply].
     move => h. exists k.
     move : h. by asimpl.
   - hauto lq:on use:Bind_Inv.
-  - move => n Γ a A B ha [i /Bind_Inv[j][h0][h1]h2].
+  - move => Γ a A B ha [i /Bind_Inv[j][h0][h1]h2].
     exists j. have : Γ ⊢ PProj PL a ∈ A by qauto use:T_Proj1.
     move : substing_wt h1; repeat move/[apply].
     by asimpl.
-  - move => s Γ P a b c i + ? + *. clear. move => h ha. exists i.
+  - move => Γ P a b c i + ? + *. clear. move => h ha. exists i.
     hauto lq:on use:substing_wt.
   - sfirstorder.
   - sfirstorder.
   - sfirstorder.
-  - move => n Γ i p A0 A1 B0 B1 hΓ ihΓ hA0
+  - move => Γ i p A0 A1 B0 B1 hΓ ihΓ hA0
              [i0 ihA0] hA [ihA [ihA' [i1 ihA'']]].
-    move => hB [ihB0 [ihB1 [i2 ihB2]]].
     repeat split => //=.
     qauto use:T_Bind.
     apply T_Bind; eauto.
+    sfirstorder.
     apply : ctx_eq_subst_one; eauto using Su_Eq, E_Symmetric.
-    eauto using T_Univ.
+    hauto lq:on.
   - hauto lq:on ctrs:Wt,Eq.
-  - move => n Γ i b0 b1 a0 a1 A B hP _ hb [ihb0 [ihb1 [i0 ihb2]]]
+  - move => n i b0 b1 a0 a1 A B hP _ hb [ihb0 [ihb1 [i0 ihb2]]]
              ha [iha0 [iha1 [i1 iha2]]].
     repeat split.
     qauto use:T_App.
@@ -680,15 +679,16 @@ Proof.
     hauto lq:on ctrs:Wt,Eq,LEq lq:on use:Bind_Inv, substing_wt.
   - hauto lq:on use:bind_inst db:wt.
   - hauto lq:on use:Bind_Inv db:wt.
-  - move => n Γ i a b A B hS _ hab [iha][ihb][j]ihs.
+  - move => Γ i a b A B hS _ hab [iha][ihb][j]ihs.
     repeat split => //=; eauto with wt.
     apply : T_Conv; eauto with wt.
     move /E_Symmetric /E_Proj1 in hab.
     eauto using bind_inst.
     move /T_Proj1 in iha.
     hauto lq:on ctrs:Wt,Eq,LEq use:Bind_Inv, substing_wt.
-  - move => n Γ P0 P1 a0 a1 b0 b1 c0 c1 i _ _ hPE [hP0 [hP1 _]] hae [ha0 [ha1 _]] _ [hb0 [hb1 hb2]] _ [hc0 [hc1 hc2]].
+  - move => Γ P0 P1 a0 a1 b0 b1 c0 c1 i _ _ hPE [hP0 [hP1 _]] hae [ha0 [ha1 _]] _ [hb0 [hb1 hb2]] _ [hc0 [hc1 [j hc2]]].
     have wfΓ : ⊢ Γ by hauto use:wff_mutual.
+    have wfΓ' : ⊢ (PNat :: Γ) by qauto use:Wff_Cons', T_Nat'.
     repeat split. by eauto using T_Ind.
     apply : T_Conv. apply : T_Ind; eauto.
     apply : T_Conv; eauto.
@@ -696,13 +696,12 @@ Proof.
     apply : T_Conv.  apply : ctx_eq_subst_one; eauto.
     by eauto using Su_Eq, E_Symmetric.
     eapply renaming; eauto.
-    eapply morphing; eauto 20 using Su_Eq, morphing_ext, morphing_id with wt.
-    apply morphing_ext; eauto.
-    replace (funcomp VarPTm shift) with (funcomp (@ren_PTm n _ shift) VarPTm); last by asimpl.
-    apply : morphing_ren; eauto using Wff_Cons' with wt.
-    apply : renaming_shift; eauto. by apply morphing_id.
-    apply T_Suc. apply T_Var'. by asimpl. apply : Wff_Cons'; eauto using T_Nat'.
-    apply : Wff_Cons'; eauto. apply : renaming_shift; eauto.
+    eapply morphing. apply : Su_Eq. apply hPE. apply wfΓ'.
+    apply morphing_ext.
+    replace (funcomp VarPTm shift) with (funcomp (@ren_PTm shift) VarPTm); last by asimpl.
+    apply : morphing_ren; eauto using morphing_id, renaming_shift.
+    apply T_Suc. apply T_Var=>//. apply here. apply : Wff_Cons'; eauto using T_Nat'.
+    apply renaming_shift.
     have /E_Symmetric /Su_Eq : Γ ⊢ PBind PSig PNat P0 ≡ PBind PSig PNat P1 ∈ PUniv i by eauto with wt.
     move /E_Symmetric in hae.
     by eauto using Su_Sig_Proj2.
@@ -711,62 +710,62 @@ Proof.
   - hauto lq:on ctrs:Wt.
   - hauto q:on use:substing_wt db:wt.
   - hauto l:on use:bind_inst db:wt.
-  - move => n Γ P i b c hP _ hb _ hc _.
+  - move => Γ P i b c hP _ hb _ hc _.
     have ? : ⊢ Γ by hauto use:wff_mutual.
     repeat split=>//.
     by eauto with wt.
     sauto lq:on use:substing_wt.
-  - move => s Γ P a b c i hP _ ha _ hb _ hc _.
+  - move => Γ P a b c i hP _ ha _ hb _ hc _.
     have ? : ⊢ Γ by hauto use:wff_mutual.
     repeat split=>//.
     apply : T_Ind; eauto with wt.
-    set Ξ : fin (S (S _)) -> _ := (X in X ⊢ _ ∈ _) in hc.
+    set Ξ := (X in X ⊢ _ ∈ _) in hc.
     have : morphing_ok Γ Ξ (scons (PInd P a b c) (scons a VarPTm)).
     apply morphing_ext. apply morphing_ext. by apply morphing_id.
     by eauto. by eauto with wt.
     subst Ξ.
     move : morphing_wt hc; repeat move/[apply]. asimpl. by apply.
     sauto lq:on use:substing_wt.
-  - move => n Γ b A B i hΓ ihΓ hP _ hb [i0 ihb].
+  - move => Γ b A B i hP _ hb [i0 ihb].
     repeat split => //=; eauto with wt.
-    have {}hb : funcomp (ren_PTm shift) (scons A Γ) ⊢ ren_PTm shift b ∈ ren_PTm shift (PBind PPi A B)
+    have {}hb : (cons A Γ) ⊢ ren_PTm shift b ∈ ren_PTm shift (PBind PPi A B)
                         by hauto lq:on use:weakening_wt, Bind_Inv.
     apply : T_Abs; eauto.
-    apply : T_App'; eauto; rewrite-/ren_PTm.
-    by asimpl.
+    apply : T_App'; eauto; rewrite-/ren_PTm. asimpl. by rewrite subst_scons_id.
     apply T_Var. sfirstorder use:wff_mutual.
+    apply here.
   - hauto lq:on ctrs:Wt.
-  - move => n Γ A B C hA [i [ihA0 ihA1]] hC [j [ihC0 ihC1]].
+  - move => Γ A B C hA [i [ihA0 ihA1]] hC [j [ihC0 ihC1]].
     have ? : ⊢ Γ by sfirstorder use:wff_mutual.
     exists (max i j).
     have [? ?] : i <= Nat.max i j /\ j <= Nat.max i j by lia.
     qauto l:on use:T_Conv, Su_Univ.
-  - move => n Γ i j hΓ *. exists (S (max i j)).
+  - move => Γ i j hΓ *. exists (S (max i j)).
     have [? ?] : S i <= S (Nat.max i j) /\ S j <= S (Nat.max i j) by lia.
     hauto lq:on ctrs:Wt,LEq.
-  - move => n Γ A0 A1 B0 B1 i hΓ ihΓ hA0 _ hA1 [i0][ih0]ih1 hB[j0][ihB0]ihB1.
+  - move => Γ A0 A1 B0 B1 i hA0 _ hA1 [i0][ih0]ih1 hB[j0][ihB0]ihB1.
     exists (max i0 j0).
     split; eauto with wt.
     apply T_Bind'; eauto.
     sfirstorder use:ctx_eq_subst_one.
-  - move => n Γ A0 A1 B0 B1 i hΓ ihΓ hA1 _ hA0 [i0][ihA0]ihA1 hB[i1][ihB0]ihB1.
+  - move => n A0 A1 B0 B1 i hA1 _ hA0 [i0][ihA0]ihA1 hB[i1][ihB0]ihB1.
     exists (max i0 i1). repeat split; eauto with wt.
     apply T_Bind'; eauto.
     sfirstorder use:ctx_eq_subst_one.
   - sfirstorder.
-  - move => n Γ A0 A1 B0 B1 _ [i][ih0 ih1].
+  - move => Γ A0 A1 B0 B1 _ [i][ih0 ih1].
     move /Bind_Inv : ih0 => [i0][h _].
     move /Bind_Inv : ih1 => [i1][h' _].
     exists (max i0 i1).
     have [? ?] : i0 <= Nat.max i0 i1 /\ i1 <= Nat.max i0 i1 by lia.
     eauto using Cumulativity.
-  - move => n Γ A0 A1 B0 B1 _ [i][ih0 ih1].
+  - move => Γ A0 A1 B0 B1 _ [i][ih0 ih1].
     move /Bind_Inv : ih0 => [i0][h _].
     move /Bind_Inv : ih1 => [i1][h' _].
     exists (max i0 i1).
     have [? ?] : i0 <= Nat.max i0 i1 /\ i1 <= Nat.max i0 i1 by lia.
     eauto using Cumulativity.
-  - move => n Γ a0 a1 A0 A1 B0 B1 /Su_Pi_Proj1 hA1.
+  - move => Γ a0 a1 A0 A1 B0 B1 /Su_Pi_Proj1 hA1.
     move => [i][ihP0]ihP1.
     move => ha [iha0][iha1][j]ihA1.
     move /Bind_Inv :ihP0 => [i0][ih0][ih0' _].
@@ -779,7 +778,7 @@ Proof.
       move : substing_wt ih0';repeat move/[apply]. by asimpl.
     + apply Cumulativity with (i := i1); eauto.
       move : substing_wt ih1' iha1;repeat move/[apply]. by asimpl.
-  - move => n Γ a0 a1 A0 A1 B0 B1 /Su_Sig_Proj1 hA1.
+  - move => Γ a0 a1 A0 A1 B0 B1 /Su_Sig_Proj1 hA1.
     move => [i][ihP0]ihP1.
     move => ha [iha0][iha1][j]ihA1.
     move /Bind_Inv :ihP0 => [i0][ih0][ih0' _].
@@ -795,23 +794,25 @@ Proof.
       Unshelve. all: exact 0.
 Qed.
 
-Lemma Var_Inv n Γ (i : fin n) A :
+Lemma Var_Inv Γ (i : nat) B A :
   Γ ⊢ VarPTm i ∈ A ->
-  ⊢ Γ /\ Γ ⊢ Γ i ≲ A.
+  lookup i Γ B ->
+  ⊢ Γ /\ Γ ⊢ B ≲ A.
 Proof.
   move E : (VarPTm i) => u hu.
   move : i E.
-  elim : n Γ u A / hu=>//=.
-  - move => n Γ i hΓ i0 [?]. subst.
+  elim : Γ u A / hu=>//=.
+  - move => i Γ A hΓ hi i0 [?]. subst.
     repeat split => //=.
-    have h : Γ ⊢ VarPTm i ∈ Γ i by eauto using T_Var.
+    have ? : A = B  by eauto using lookup_deter. subst.
+    have h : Γ ⊢ VarPTm i ∈ B by eauto using T_Var.
     eapply regularity in h.
     move : h => [i0]?.
     apply : Su_Eq. apply E_Refl; eassumption.
   - sfirstorder use:Su_Transitive.
 Qed.
 
-Lemma renaming_su' : forall n m Δ Γ (ξ : fin n -> fin m) (A B : PTm n) u U ,
+Lemma renaming_su' : forall Δ Γ ξ (A B : PTm) u U ,
     u = ren_PTm ξ A ->
     U = ren_PTm ξ B ->
     Γ ⊢ A ≲ B ->
@@ -819,23 +820,23 @@ Lemma renaming_su' : forall n m Δ Γ (ξ : fin n -> fin m) (A B : PTm n) u U ,
     Δ ⊢ u ≲ U.
 Proof. move => > -> ->. hauto l:on use:renaming. Qed.
 
-Lemma weakening_su : forall n Γ (A0 A1 B : PTm n) i,
+Lemma weakening_su : forall Γ (A0 A1 B : PTm) i,
     Γ ⊢ B ∈ PUniv i ->
     Γ ⊢ A0 ≲ A1 ->
-    funcomp (ren_PTm shift) (scons B Γ) ⊢ ren_PTm shift A0 ≲ ren_PTm shift A1.
+    (cons B Γ) ⊢ ren_PTm shift A0 ≲ ren_PTm shift A1.
 Proof.
-  move => n Γ A0 A1 B i hB hlt.
+  move => Γ A0 A1 B i hB hlt.
   apply : renaming_su'; eauto.
   apply : Wff_Cons'; eauto.
   apply : renaming_shift; eauto.
 Qed.
 
-Lemma regularity_sub0 : forall n Γ (A B : PTm n), Γ ⊢ A ≲ B -> exists i, Γ ⊢ A ∈ PUniv i.
+Lemma regularity_sub0 : forall Γ (A B : PTm), Γ ⊢ A ≲ B -> exists i, Γ ⊢ A ∈ PUniv i.
 Proof. hauto lq:on use:regularity. Qed.
 
-Lemma Su_Pi_Proj2_Var n Γ (A0 A1 : PTm n) B0 B1 :
+Lemma Su_Pi_Proj2_Var Γ (A0 A1 : PTm) B0 B1 :
   Γ ⊢ PBind PPi A0 B0 ≲ PBind PPi A1 B1 ->
-  funcomp (ren_PTm shift) (scons A1 Γ) ⊢ B0 ≲ B1.
+  cons A1 Γ ⊢ B0 ≲ B1.
 Proof.
   move => h.
   have /Su_Pi_Proj1 h1 := h.
@@ -843,15 +844,16 @@ Proof.
   move /weakening_su : (h) h2. move => /[apply].
   move => h2.
   apply : Su_Pi_Proj2'; try eassumption; rewrite -?/ren_PTm; cycle 2.
-  apply E_Refl. apply T_Var' with (i := var_zero); eauto.
+  apply E_Refl. apply T_Var with (i := var_zero); eauto.
   sfirstorder use:wff_mutual.
-  by asimpl.
-  by asimpl.
+  apply here.
+  by asimpl; rewrite subst_scons_id.
+  by asimpl; rewrite subst_scons_id.
 Qed.
 
-Lemma Su_Sig_Proj2_Var n Γ (A0 A1 : PTm n) B0 B1 :
+Lemma Su_Sig_Proj2_Var Γ (A0 A1 : PTm) B0 B1 :
   Γ ⊢ PBind PSig A0 B0 ≲ PBind PSig A1 B1 ->
-  funcomp (ren_PTm shift) (scons A0 Γ) ⊢ B0 ≲ B1.
+  (cons A0 Γ) ⊢ B0 ≲ B1.
 Proof.
   move => h.
   have /Su_Sig_Proj1 h1 := h.
@@ -859,8 +861,9 @@ Proof.
   move /weakening_su : (h) h2. move => /[apply].
   move => h2.
   apply : Su_Sig_Proj2'; try eassumption; rewrite -?/ren_PTm; cycle 2.
-  apply E_Refl. apply T_Var' with (i := var_zero); eauto.
+  apply E_Refl. apply T_Var with (i := var_zero); eauto.
   sfirstorder use:wff_mutual.
-  by asimpl.
-  by asimpl.
+  apply here.
+  by asimpl; rewrite subst_scons_id.
+  by asimpl; rewrite subst_scons_id.
 Qed.
